Preservation for fun : nil case

LocalLang/TypingGuarantees.lean
@@ -3,13 +3,61 @@ import LocalLang.Semantics
 import LocalLang.Types
 import LocalLang.Typing
 
-def EnvRespectsCtx (Γ : TypeContext) (V : Env) : Prop := sorry
+def EnvRespectsCtx (Γ : TypeContext) (V : Env) : Prop :=
+  ∀ (x : String) (n : ℕ), V[x]? = some n → Γ[x]? = LLType.nat
+
+def CtxRespectsEnv (V : Env) (Γ : TypeContext) : Prop :=
+  ∀ x : String, Γ[x]? = some LLType.nat → x ∈ V
+
+def CtxRespectsDefs (Γ : TypeContext) (defs : Definitions) : Prop :=
+   (T_ret : LLType) → (arg_types : List LLType) → (f : String) → (f_in_defs : f ∈ defs) →
+    (h_type : Γ[f]? = some (LLType.func arg_types T_ret)) →
+    (TypeJdg Γ defs[f].body T_ret)
+
+
+theorem addBindings_typing {ps : List String} {es : List Expr} {bd : Expr}
+                                {T_ret : LLType} {arg_types : List LLType}
+  {defs : Definitions} (ctxRespectDefs : CtxRespectsDefs Γ defs)
+  (f : String) (h_args : Γ[f]? = some (LLType.func arg_types T_ret))
+  (f_in_defs : f ∈ defs) (eq_bd_defs : bd = defs[f].body)
+  : TypeJdg Γ (Expr.addBindings (ps.zip es) bd) T_ret
+    := by induction ps with
+      | nil =>
+        simp [Expr.addBindings]
+        let res := ctxRespectDefs T_ret arg_types f f_in_defs h_args
+        rw [eq_bd_defs.symm] at res
+        apply res
+      | cons head tail ih =>
+        sorry
+
 
 -- TODO: prove
 -- TODO: V and Γ should be related
-theorem preservation (Γ : TypeContext) (e e' : Expr) (ty : LLType)
+theorem preservation (Γ : TypeContext) (e e' : Expr) (ty : LLType) (defs : Definitions)
     (h_env_respects : EnvRespectsCtx Γ V)
-  : Expr.TypeJdg Γ e ty → HeadSmallStep V e e' → Expr.TypeJdg Γ e' ty := sorry
+  : TypeJdg Γ e ty → HeadSmallStep defs V e e' → TypeJdg Γ e' ty := by
+  intro h_jdg b
+  induction b
+  · cases h_jdg
+    · rename_i x n a relΓ
+      unfold EnvRespectsCtx at h_env_respects
+      let ent_ctx_link := h_env_respects x n a
+      let symmRelΓ := relΓ.symm
+      have ty_eq := Option.some.inj (symmRelΓ.trans ent_ctx_link)
+      rw [ty_eq]
+      constructor
+  · cases h_jdg
+    · rename_i H₁ H₂
+      apply TypeJdg.jdg_const
+  · rename_i name val n
+    cases h_jdg
+    · rename_i H₁ H₂
+      cases H₂
+      constructor
+  · cases h_jdg
+    rename_i f es' ps bd f_in_defs a eq_bd_defs es eq arg_types h_f h_args
+    simp [es]
+    apply addBindings_typing ctx_defs_respects f h_args f_in_defs eq_bd_defs
 
 -- Progress: if TypeJdg Γ e ty, then e can take a step.
 -- TODO: formalize
