LocalLang/Typing.lean
@@ -9,6 +9,7 @@ mutual
     | jdg_closure {ps bd argTs retTy} : Expr.TypeJdg (.ofList (ps.zip argTs)) bd retTy →
       ps.length = argTs.length → Value.TypeJdg (.closure ps bd) (.func argTs retTy)
 
+
   inductive Expr.TypeJdg : TypeContext → Expr → LLType → Prop where
     | jdg_value {ty} : Value.TypeJdg v ty → Expr.TypeJdg Γ (.value v) ty
     | jdg_var {Γ : TypeContext} {name : String} {ty : LLType} (H : Γ[name]? = some ty)
@@ -17,7 +18,7 @@ mutual
     | jdg_fun {Γ : TypeContext} {es : List Expr} {arg_types : List LLType} {T_return : LLType}
                   (f_jdg : Expr.TypeJdg Γ f (.func arg_types T_return))
                   (H_args : Expr.TypeJdgList Γ es arg_types)
-                        : Expr.TypeJdg Γ (.funCall f es) (LLType.func arg_types T_return)
+                        : TypeJdg Γ (.funCall f es) T_return
     | jdg_binOp {Γ : TypeContext} {op : BinOp} {e₁ e₂ : Expr}
                 (H₁ : Expr.TypeJdg Γ e₁ LLType.nat) (H₂ : Expr.TypeJdg Γ e₂ LLType.nat)
                         : Expr.TypeJdg Γ (.binOp op e₁ e₂) .nat
